---
title: Matrix (2)
author:
  name: luo-songtao
  link: https://github.com/luo-songtao
date: 2021-02-20 08:00:00 +0800
categories: [Mathematics, Algebra, Matrix]
tags: [Matrix, Inverse Matrix]
math: true
mermaid: true
---


## 矩阵的特征



### 逆矩阵恒等式



#### Identity-1

$$\begin{aligned} (I+P)^{-1} = I-(I+P)^{-1}P = I-P(I+P)^{-1} \end{aligned}$$

- **Proof-Identity-1**

  $$\begin{aligned} &I = (I+P)^{-1}(I+P) = (I+P)^{-1}+(I+P)^{-1}P \\  \Longrightarrow & (I+P)^{-1} = I-(I+P)^{-1}P = I-P(I+P)^{-1} \end{aligned}$$

#### Identity-2：Push-Through Identity

$$\begin{aligned} (I+AB)^{-1}A = A(I+BA)^{-1} \end{aligned}$$

- **Proof-Identity-2**

  $$\begin{aligned} &A(I+BA) = (I+AB)A \\ \Longrightarrow&  (I+AB)^{-1}A(I+BA)(I+BA)^{-1} = (I+AB)^{-1}(I+AB)A(I+BA)^{-1} \\ \Longrightarrow & (I+AB)^{-1}A = A(I+BA)^{-1} \end{aligned}$$

#### Identity-3

$$\begin{aligned} (I+AB)^{-1} = I-A(I+BA)^{-1}B \end{aligned}$$

- **Proof-Identity-3**

  $$\begin{aligned} &根据Identity-1和Identity-2 \\ \Longrightarrow  & (I+AB)^{-1} = I-(I+AB)^{-1}AB = I - A(I+BA)^{-1}B \end{aligned}$$

#### Identity-4

$$\begin{aligned} B+BDCA^{-1}B = BD(D^{-1}+CA^{-1}B) = (A+BDC)A^{-1}B \end{aligned}$$

#### Identity-5

$$\begin{aligned} (A+BDC)^{-1}BD = A^{-1}B(D^{-1}+CA^{-1}B)^{-1} \end{aligned}$$

- **Proof-Identity-5**：方法同Identity-2

- **Identity-5**的变种形式（假设对应的矩阵大小都是正确合适的）：

  $$\begin{aligned} &\bullet (A+B^TDC)^{-1}B^TD = A^{-1}B^T(D^{-1}+CA^{-1}B^T)^{-1} \\ &\bullet (A+B^TDB)^{-1}B^TD = A^{-1}B^T(D^{-1}+BA^{-1}B^T)^{-1} \end{aligned}$$

#### Identity-6：Woodbury-Matrix-Identity

$$\begin{aligned} (A+BDC)^{-1} = A^{-1} - A^{-1}B(D^{-1}+CA^{-1}B)^{-1}CA^{-1} \end{aligned}$$

- **Proof-Lemma-6**

$$\begin{aligned} A^{-1} &= (A+BDC)^{-1}(A+BDC)A^{-1} \\ &= (A+BDC)^{-1}(I+BDCA^{-1}) \\&=  (A+BDC)^{-1} + (A+BDC)^{-1}BDCA^{-1} \qquad 使用identity-5 \\ &= (A+BDC)^{-1}+ A^{-1}B(D^{-1}+CA^{-1}B)^{-1}CA^{-1} \end{aligned}$$















